bit rev shuffle proof more complicated than expected

lib/falcon/ntt_index.dfy
@@ -24,6 +24,25 @@ module ntt_index {
             ToNatRight(rs)
     }
 
+    lemma bit_rev_int_basics_lemma(len: pow2_t)
+        requires len.full >= 4;
+        ensures bit_rev_int(0, len) == 0;
+        ensures bit_rev_int(1, len) != 1;
+    {
+        assume len.exp >= 2;
+        reveal Pow2();
+        var zero := FromNatWithLen(0, len.exp);
+        LemmaSeqZero(zero);
+        var zrs := Reverse(zero);
+        assert zrs == SeqZero(len.exp);
+
+        var one := FromNatWithLen(1, len.exp);
+        var ors := Reverse(one);
+
+        assume ors != one;
+        LemmaSeqNeq(ors, one);
+    }
+
     lemma bit_rev_int_lemma0(i: nat, bound: pow2_t)
         requires i < bound.full;
         ensures bit_rev_int(i, pow2_double(bound)) == 2 * bit_rev_int(i, bound);
@@ -212,4 +231,556 @@ module ntt_index {
             bit_rev_int(i, bound) + bound.full;
         }
     }
+    
+    predicate {:opaque} is_bit_rev_shuffle<T>(a: seq<T>, b: seq<T>, len: pow2_t)
+        requires |a| == |b| == len.full;
+    {
+        forall i | 0 <= i < len.full ::
+            a[i] ==  b[bit_rev_int(i, len)]
+    }
+
+    lemma bit_rev_symmetric(i: nat, bound: pow2_t)
+        requires i < bound.full;
+        ensures bit_rev_int(bit_rev_int(i, bound), bound) == i;
+    {
+        if bound.exp != 0 {
+            reveal Pow2();
+            var s := FromNatWithLen(i, bound.exp);
+            var rs := Reverse(s);
+            var rrs := Reverse(rs); 
+            var rbi := bit_rev_int(i, bound);
+            assert rbi == ToNatRight(rs);
+
+            assert FromNatWithLen(rbi, bound.exp) == rs by {
+                LemmaSeqEq(rs, FromNatWithLen(rbi, bound.exp));
+            }
+
+            calc == {
+                bit_rev_int(rbi, bound);
+                ToNatRight(Reverse(rs));
+                ToNatRight(Reverse(rs));
+                ToNatRight(rrs);
+                {
+                    ReverseSymmetric(s);
+                    assert rrs == s;
+                }
+                ToNatRight(s);
+            }
+        }
+    }
+
+    lemma bit_rev_shuffle_symmetric<T>(a: seq<T>, b: seq<T>, len: pow2_t)
+        requires |a| == |b| == len.full;
+        requires is_bit_rev_shuffle(a, b, len);
+        ensures is_bit_rev_shuffle(b, a, len);
+    {
+        reveal is_bit_rev_shuffle();
+        forall i | 0 <= i < len.full
+            ensures b[i] == a[bit_rev_int(i, len)]
+        {
+            var j := bit_rev_int(i, len);
+            calc == {
+                b[i];
+                {
+                    bit_rev_symmetric(i, len);
+                }
+                b[bit_rev_int(j, len)];
+                a[j];
+            }
+        }
+    }
+
+    predicate {:opaque} is_set_min(x: nat, s: set<nat>)
+    {
+        forall t | t in s :: x <= t
+    }
+
+    function {:opaque} minimum(s: set<nat>): (x: nat)
+        requires |s| >= 1;
+        ensures is_set_min(x, s);
+        ensures x in s;
+    {
+        reveal is_set_min();
+        var y :| y in s;
+        var s' := s - {y};
+
+        if |s| == 1 then
+            assert y in s;
+            assert |s'| == 0;
+            assert s' == {};
+            assert s == {y};
+            y
+        else 
+            var m := minimum(s');
+            var x := (if y < m then y else m);
+            assert is_set_min(x, s) by {
+                forall t | t in s
+                    ensures x <= t
+                {
+                    if t in s' {
+                        assert x <= m <= t;
+                    } else {
+                        assert x <= y;
+                    }
+                }
+            }
+            x
+    }
+
+    // lemma set_min_uiique(s: set<nat>): (x: nat)
+    // {
+    datatype rev_view = rev_view(
+        finished: set<nat>,
+        unfinished: set<nat>,
+        len: pow2_t)
+    {
+        predicate {:opaque} rev_view_wf()
+        {
+            && (forall bi | (bi in finished || bi in unfinished) ::
+                0 <= bi < len.full)
+            && (finished !! unfinished)
+            && (finished + unfinished == set bi | 0 <= bi < len.full :: bi)
+            && len.full >= 4
+        }
+
+        lemma buff_index_state_lemma(bi: nat)
+            requires bi < len.full;
+            requires rev_view_wf();
+            ensures (bi in finished) != (bi in unfinished)
+        {
+            reveal rev_view_wf();
+            if bi in finished {
+                assert bi !in unfinished;
+            }
+            if bi in unfinished {
+                assert bi !in finished;
+            }
+        }
+  
+        lemma rev_entry_wf_lemma(bi: nat)
+            requires rev_view_wf();
+            requires bi in finished || bi in unfinished;
+            ensures bi < len.full
+        {
+            reveal rev_view_wf();
+        }
+    
+        predicate index_is_shuffled<T>(a: seq<T>, b: seq<T>, bi: nat)
+            requires bi < len.full;
+            requires |a| == |b| == len.full;
+            requires rev_view_wf();
+        {
+            var rbi := bit_rev_int(bi, len);
+            && a[bi] == b[rbi]
+            && a[rbi] == b[bi]
+        }
+
+        function get_split_index(): (bi: nat)
+            requires |unfinished| != 0;
+            requires rev_view_wf();
+            ensures bi < len.full;
+            ensures bi !in finished;
+        {
+            var bi := minimum(unfinished);
+            rev_entry_wf_lemma(bi);
+            buff_index_state_lemma(bi);
+            bi
+        }
+
+        predicate {:opaque} partially_shuffled_inv<T>(a: seq<T>, b: seq<T>)
+            requires |a| == |b| == len.full;
+            ensures partially_shuffled_inv(a, b) ==> rev_view_wf();
+        {
+            && rev_view_wf()
+            && reveal rev_view_wf();
+            && |unfinished| != 0
+            && var split_index := get_split_index();
+            && (forall bi | bi in finished :: bit_rev_int(bi, len) in finished)
+            && (forall bi | bi in unfinished :: bit_rev_int(bi, len) in unfinished)
+            && (forall bi | bi in finished :: index_is_shuffled(a, b, bi))
+            && (forall bi | 0 <= bi < split_index :: bi in finished)
+        }
+
+        static function init_finished(len: pow2_t): set<nat>
+            requires len.full >= 4;
+        {
+            set bi: nat | (0 <= bi < len.full && bi == bit_rev_int(bi, len)) :: bi
+        }
+
+        static function init_unfinished(len: pow2_t): set<nat>
+            requires len.full >= 4;
+        {
+            set bi: nat | (0 <= bi < len.full && bi != bit_rev_int(bi, len)) :: bi
+        }
+
+        static function {:opaque} init_rev_view<T>(a: seq<T>, len: pow2_t): (r: rev_view)
+            requires |a| == len.full >= 4;
+            ensures r.len == len;
+            // ensures r.partially_shuffled_inv(a, a);
+        {    
+            var finished := rev_view.init_finished(len);
+            var unfinished := rev_view.init_unfinished(len);
+            rev_view(finished, unfinished, len)
+        }
+
+        static lemma init_unfinished_lemma(len: pow2_t)
+            requires len.full >= 4;
+            ensures 1 in init_unfinished(len);
+            ensures |init_unfinished(len)| != 0;
+            ensures minimum(init_unfinished(len)) == 1;
+        {
+            var unfinished := init_unfinished(len);
+            bit_rev_int_basics_lemma(len);
+            assert 1 in unfinished;
+            assert |unfinished| != 0;
+            assert |unfinished| >= 1;
+            assume minimum(init_unfinished(len)) == 1;
+        }
+
+        lemma init_rev_view_inv_lemma<T>(a: seq<T>, len: pow2_t)
+            requires |a| == len.full >= 4;
+            requires this == init_rev_view(a, len);
+        {
+            reveal init_rev_view();
+
+            assert finished !! unfinished;
+            assert finished + unfinished == set bi | 0 <= bi < len.full :: bi;
+
+            bit_rev_int_basics_lemma(len);
+
+            forall bi | bi in finished
+                ensures bit_rev_int(bi, len) in finished
+            {}
+
+            forall bi | bi in unfinished 
+                ensures bit_rev_int(bi, len) in unfinished;
+            {
+                var bri := bit_rev_int(bi, len);
+                if  bri !in unfinished {
+                    assert bri in finished;
+                    assert bit_rev_int(bri, len) in finished;
+                    bit_rev_symmetric(bi, len);
+                    assert bi in finished;
+                    assert false;
+                }
+            }
+
+            forall bi | bi in finished
+                ensures index_is_shuffled(a, a, bi)
+            {}
+
+            assert rev_view_wf() by {
+                reveal rev_view_wf();
+            }
+
+
+            init_unfinished_lemma(len);
+            var split_index := get_split_index();
+            assume split_index == 1;
+  
+            forall bi | 0 <= bi < split_index
+                ensures bi in finished
+            {
+                assert bi == 0;
+                assert bit_rev_int(0, len) == 0;
+            }
+        }
+
+        // function next_rev_view<T>(a: seq<T>, b: seq<T>): (r: rev_view)
+        //     requires |unfinished| != 0;
+        //     requires |a| == |b| == len.full;
+        //     requires partially_shuffled_inv(a, b);
+        // {
+        //     var bi :=  get_split_index();
+        //     rev_view(finished + {bi, bit_rev_int(bi, len)},
+        //         unfinished - {bi, bit_rev_int(bi, len)},
+        //         len)
+        // }
+
+        // lemma next_rev_view_lemma<T>(a: seq<T>, b: seq<T>, bj: nat, r: rev_view)
+        //     requires bj < |a| == |b| == len.full;
+        //     requires partially_shuffled_inv(a, b, bj);
+        //     requires bj !in finished;
+        //     requires r == next_rev_view(a, b, bj);
+        // {
+        //     // var rbj := bit_rev_int(bj, len);
+        //     // var c := b[bj := c[rbj]][rbj := c[bj]];
+
+        //     // assert r.partially_shuffled_inv(a, c, bj);
+
+        // }
+    }
+
+    datatype rev_table = rev_table(
+        table: seq<(nat, nat)>,
+        len: pow2_t)
+    {
+        predicate table_entry_wf(ti: nat)
+            requires ti < |table|;
+        {
+            && ti <= table[ti].0
+            && table[ti].0 < len.full
+            && table[ti].1 < len.full
+            && table[ti].0 == bit_rev_int(table[ti].1, len)
+            && table[ti].1 == bit_rev_int(table[ti].0, len)
+        }
+
+        predicate {:opaque} rev_table_wf()
+            ensures rev_table_wf() ==> len.full >= 4
+            ensures rev_table_wf() ==> |table| >= 2
+        {
+            && (forall ti | 0 <= ti < |table| :: table_entry_wf(ti))
+            // table is sorted in terms of the key (src) index
+            && (forall ti, tj | 0 <= ti < tj < |table| :: table[ti].0 < table[tj].0)
+            && len.full >= 4
+            && |table| >= 2
+        }
+
+        lemma table_entry_wf_lemma(ti: nat)
+            requires 0 <= ti < |table|
+            requires rev_table_wf();
+            ensures table_entry_wf(ti);
+        {
+            reveal rev_table_wf();
+        }
+
+        // bi is a buffer index (NOT a table index)
+        predicate in_table(bi: nat)
+            requires bi < len.full;
+        {
+            exists ti: nat :: (
+                ti < |table| && table[ti].0 == bi)
+        }
+
+        // given a (bi) buffer index, return the (ti) table index 
+        function get_table_index(bi: nat): (ti: nat)
+            requires rev_table_wf();
+            requires bi < len.full;
+            requires in_table(bi);
+            ensures ti < |table|;
+            ensures table_entry_wf(ti);
+        {
+            var ti: nat :| (ti < |table| && table[ti].0 == bi);
+            table_entry_wf_lemma(ti);
+            ti
+        }
+
+        function get_buffer_index(ti: nat): (bi: nat)
+            requires rev_table_wf();
+            requires ti < |table|;
+            ensures table_entry_wf(ti);
+        {
+            table_entry_wf_lemma(ti);
+            table[ti].0
+        }
+
+        function buffer_prefix_index(ti: nat): nat 
+            requires rev_table_wf();
+            requires ti <= |table|;
+        {
+            if ti == |table| then len.full else get_buffer_index(ti)
+        }
+
+        predicate prefix_prev_bi_properties(ti: nat, bi: nat)
+            requires rev_table_wf();
+            requires ti < |table|;
+            requires bi < buffer_prefix_index(ti);
+        {
+            var split_index := buffer_prefix_index(ti);
+            var rbi := bit_rev_int(bi, len);
+            && (!in_table(bi) ==> (
+                || (bi == rbi)
+                || (in_table(rbi) && 0 <= rbi < split_index)))
+            && (in_table(bi) ==> 
+                && (bi != rbi)
+                && (!in_table(rbi)))
+        }
+
+        predicate bit_rev_table_prefix_inv(ti: nat)
+            requires ti < |table|;
+            requires rev_table_wf();
+        {
+            var split_index := buffer_prefix_index(ti);
+            forall bi | (0 <= bi < split_index) ::
+                prefix_prev_bi_properties(ti, bi)
+        }
+
+        predicate {:opaque} bit_rev_table_inv()
+            ensures bit_rev_table_inv() ==> rev_table_wf()
+        {
+            && rev_table_wf()
+            && (forall ti | 0 <= ti < |table| :: 
+                bit_rev_table_prefix_inv(ti))
+        }
+
+        // lemma partially_shuffled_inv_peri_lemma<T>(
+        //     a: seq<T>, b: seq<T>, c: seq<T>,
+        //     ti: nat, i: nat, j: nat,
+        //     view: rev_view)
+        //     requires |a| == |b| == |c| == len.full;
+        //     requires ti < |table|;
+        //     requires bit_rev_table_inv();
+        //     requires buffer_prefix_index(ti) < len.full;
+        //     requires view.len == len;
+        //     requires i == table[ti].0 < len.full;
+        //     requires j == table[ti].1 < len.full;
+        //     requires view.partially_shuffled_inv(a, b, buffer_prefix_index(ti));
+        //     requires c == b[i := b[j]][j := b[i]];
+        // {
+
+        // }
+
+
+        // method bit_rev<T>(a: seq<T>) returns (b: seq<T>)
+        //     requires |a| == len.full;
+        //     requires bit_rev_table_inv();
+        // {
+        //     b := a;
+        //     var ti := 0;
+
+        //     ghost var view := rev_view.init_rev_view(a, len);
+
+        //     assume buffer_prefix_index(0) == 1;
+
+        //     while ti < |table|
+        //         invariant |b| == len.full;
+        //         invariant view.
+        //             partially_shuffled_inv(a, b, buffer_prefix_index(ti));
+        //         decreases |table| - ti;
+        //     {
+        //         var prev_b := b;
+
+        //         var i := table[ti].0;
+        //         var j := table[ti].1;
+
+        //         table_entry_wf_lemma(ti);
+
+        //         var temp := b[i];
+        //         b := b[i := b[j]];
+        //         b := b[j := temp];
+
+        //         partially_shuffled_inv_peri_lemma(a, prev_b, b, ti, i, j, view);
+        //         ti := ti + 1;
+        //         assume false;
+        //     }
+        // }
+    }
 }
+
+        // lemma buffer_prefix_index_lemma<T>(a: seq<T>, bi: nat)
+        //     requires bit_rev_table_inv();
+        //     requires finished == inital_finished_set();
+        //     requires bi < len.full;
+        //     requires |a| == len.full;
+        // {
+        //     var split_index := buffer_prefix_index(0);
+        //     var ti := 0;
+
+        //     // reveal inital_finished_set();
+
+        //     reveal partially_shuffled_inv();
+        //     assert bit_rev_table_prefix_inv(ti) by {
+        //         reveal bit_rev_table_inv();
+        //     }
+  
+        //     if 0 <= bi < len.full && finished_set_membership(a, a, bi, ti) {
+        //         // assert prev_bi_properties(ti, bi);
+
+        //     //   var rbi := bit_rev_int(bi, len);
+        //     //     assert  && (!in_table(bi) ==> (
+        //     //         || (bi == rbi)
+        //     //         || (in_table(rbi) && 0 <= rbi < split_index)))
+        //     //     && (in_table(bi) ==> 
+        //     //         && (bi != rbi)
+        //     //         && (!in_table(rbi)));
+
+        //     }
+        // }
+
+        // lemma inital_finished_set_lemma<T>(a: seq<T>)
+        //     requires bit_rev_table_inv();
+        //     requires |a| == len.full;
+        //     requires finished == inital_finished_set();
+        //     // ensures partially_shuffled_inv(a, a, 0);
+        // {
+        //     reveal inital_finished_set();
+        //     reveal partially_shuffled_inv();
+
+        //     var ti := 0;
+        //     assume bit_rev_int(0, len) == 0;
+
+        //     forall bi | 0 <= bi < len.full && bi in finished
+        //         ensures finished_set_membership(a, a, bi, ti);
+        //     {
+        //         var rbi := bit_rev_int(bi, len);
+        //         var split_index := 0;
+        //         assert rbi == bi;
+        //     }
+        
+        //     assert bit_rev_table_prefix_inv(ti) by {
+        //         reveal bit_rev_table_inv();
+        //     }
+
+        //     forall bi | 0 <= bi < len.full && finished_set_membership(a, a, bi, ti)
+        //         ensures bi in finished;
+        //     {
+        //         var rbi := bit_rev_int(bi, len);
+        //         var split_index := buffer_prefix_index(ti);
+        //         assert a[bi] == a[rbi];
+        //         assert a[rbi] == a[bi];
+
+        //         if 0 <= bi < split_index {
+        //             assume false;
+        //         } else {
+        //             assert bi == bit_rev_int(bi, len); 
+        //         }
+
+        //         // assert bi == bit_rev_int(bi, len)            
+        //     }
+
+        // }
+
+        // lemma partially_shuffled_inv_lemma<T>(
+        //     a: seq<T>, b: seq<T>, c: seq<T>,
+        //     finished: set<nat>, 
+        //     ti: nat, i: nat, j: nat)
+        //     requires bit_rev_table_inv();
+        //     requires |a| == |b| == |c| == len.full;
+        //     requires ti < |table|;
+        //     requires i < len.full;
+        //     requires i == table[ti].0;
+        //     requires j < len.full;
+        //     requires j == table[ti].1;
+        //     requires partially_shuffled_inv(a, b, finished);
+        //     requires c == b[i := b[j]][j := b[i]];
+        // {
+        //     var new_finished := finished + {i, j};
+        //     reveal partially_shuffled_inv();
+        //     table_entry_wf_lemma(ti);
+
+        //     forall bi | bi in new_finished
+        //         ensures 0 <= bi < len.full
+        //     {
+        //         if bi != i && bi != j {
+        //             assert bi in finished;
+        //         }
+        //     }
+            
+        //     forall bi | 0 <= bi < len.full && bi in new_finished
+        //         ensures c[bi] == a[bit_rev_int(bi, len)]
+        //         // ensures c[bit_rev_int(bi, len)] == a[bi]
+        //     {
+        //         if bi == i {
+        //             assert c[i] == b[j];
+        //             assert j !in finished;
+        //             assume false;
+        //         } else if bi == j {
+        //             assume false;
+        //         } else {
+        //             assert c[bi] == b[bi];
+        //         }
+        //     }
+        //     // && (forall bi | 0 <= bi < len.full && bi !in finished :: (
+        //     //     && b[bi] == a[bi]))
+        // }
+
