lib/falcon/bv32_falcon_lemmas.i.dfy
@@ -688,58 +688,58 @@ module bv32_falcon_lemmas {
       assert int32_rs(to_int32(x), shift) >= 0 by { DivMod.LemmaDivBasicsAuto(); }
     }
 
-     lemma lemma_mq_rshift1_correct(par: uint32, b: uint32, c: uint32, d: uint32, r: uint32, x: int)
-         requires 0 <= x < 12289;
-         requires par == uint32_and(x, 1);
-         requires b == uint32_sub(0, par);
-         requires c == uint32_and(b, 12289);
-         requires d == uint32_add(x, c);
-         requires r == to_uint32(int32_rs(to_int32(d), 1));
- 
-         //ensures r == (x / 2) % 12289;
-         ensures IsModEquivalent(2 * r, x, 12289);
-         ensures r < 12289;
-     {
-       var Q : int := 12289;
-       assert par == 0 || par == 1 by { reveal_and(); }
- 
-       if par == 0 {
-         assert b == 0;
-         assert c == 0 by { reveal_and(); }
-         assert x % 2 == 0 by { reveal_and(); }
-         assert d == x;
-         
-         assert 0 <= to_int32(d) < Q;
-         assert r == int32_rs(to_int32(d), 1) by { lemma_positive_rs(x, 1); }
- 
-         assert r == d / Power2.Pow2(1);
-         assert r == d / 2 by { Power2.Lemma2To64(); }
- 
-         assert IsModEquivalent(r, x / 2, Q);
-         
-       } else {
-         assert b == 0xffff_ffff;
-         assert c == Q by { reveal_and(); }
-         assert d == uint32_add(x, Q);
-         assert d == x + Q;
+    lemma lemma_mq_rshift1_correct(par: uint32, b: uint32, c: uint32, d: uint32, r: uint32, x: int)
+        requires 0 <= x < 12289;
+        requires par == uint32_and(x, 1);
+        requires b == uint32_sub(0, par);
+        requires c == uint32_and(b, 12289);
+        requires d == uint32_add(x, c);
+        requires r == to_uint32(int32_rs(to_int32(d), 1));
 
-         assert 0 <= to_int32(d) <= x + Q;
-         assert r == int32_rs(to_int32(d), 1) by { lemma_positive_rs(x + Q, 1); }
+        //ensures r == (x / 2) % 12289;
+        ensures IsModEquivalent(2 * r, x, 12289);
+        ensures r < 12289;
+    {
+        var Q : int := 12289;
+        assert par == 0 || par == 1 by { reveal_and(); }
  
-         assert IsModEquivalent(d, x, Q);
- 
-         assert r == d / Power2.Pow2(1);
-         assert r == d / 2 by { Power2.Lemma2To64(); }
- 
-         assert r == (x + Q) / 2;
-         
-        //  assert x % 2 == 1 by { reveal_and(); }
-        assume x % 2 == 1;
-         assert Q % 2 == 1;
-         assert (x + Q) % 2 == 0 by { DivMod.LemmaModAdds(x, Q, 2); }
- 
-         assert r == (x + Q) / 2;
-         assert IsModEquivalent(2 * r, x + Q, Q);
-       }
-     }
+        if par == 0 {
+            assert b == 0;
+            assert c == 0 by { reveal_and(); }
+            assert x % 2 == 0 by { reveal_and(); }
+            assert d == x;
+            
+            assert 0 <= to_int32(d) < Q;
+            assert r == int32_rs(to_int32(d), 1) by { lemma_positive_rs(x, 1); }
+    
+            assert r == d / Power2.Pow2(1);
+            assert r == d / 2 by { Power2.Lemma2To64(); }
+    
+            assert IsModEquivalent(r, x / 2, Q);
+            
+        } else {
+            assert b == 0xffff_ffff;
+            assert c == Q by { reveal_and(); }
+            assert d == uint32_add(x, Q);
+            assert d == x + Q;
+
+            assert 0 <= to_int32(d) <= x + Q;
+            assert r == int32_rs(to_int32(d), 1) by { lemma_positive_rs(x + Q, 1); }
+    
+            assert IsModEquivalent(d, x, Q);
+    
+            assert r == d / Power2.Pow2(1);
+            assert r == d / 2 by { Power2.Lemma2To64(); }
+    
+            assert r == (x + Q) / 2;
+            
+            //  assert x % 2 == 1 by { reveal_and(); }
+            assume x % 2 == 1;
+            assert Q % 2 == 1;
+            assert (x + Q) % 2 == 0 by { DivMod.LemmaModAdds(x, Q, 2); }
+    
+            assert r == (x + Q) / 2;
+            assert IsModEquivalent(2 * r, x + Q, Q);
+        }
+    }
 }
